

# Model Predictive Path Integral Control: A Tutorial

Xiong Zeng

January 20, 2026

- 1 Introduction
- 2 Motivation and Optimality for Single Iteration
- 3 Convergence of MPPI for Quadratic Programming

## Introduction

Model predictive path integral (**MPPI**) control is a powerful and popular controller method in robotics and control, because

- it can handle **nonconvex** and **non-smooth** optimization problems,
- and it can be computed in **real-time** with GPU due to its **parallel computation** nature.

---

<sup>1</sup>Williams, et al. Information theoretic MPC for model-based reinforcement learning. ICRA 2017.

<sup>2</sup>Xue, et al. Full-order sampling-based mpc for torque-level locomotion control via diffusion-style annealing. ICRA 2025.

<sup>3</sup>Pan, et al. pider: Scalable physics-informed dexterous retargeting. ArXiv 2025.

<sup>4</sup>Halder et al. Trajectory Planning with Signal Temporal Logic Costs using Deterministic Path Integral Optimization. Arxiv 2025.

# Introduction

Model predictive path integral (**MPPI**) control is a powerful and popular controller method in robotics and control, because

- it can handle **nonconvex** and **non-smooth** optimization problems,
- and it can be computed in **real-time** with GPU due to its **parallel computation** nature.

Many applications:

- Aggressive driving <sup>1</sup>
- Legged robot control<sup>2</sup>
- Sim2real dexterous retargeting <sup>3</sup>
- Hard control problems in my research (MPPI > Policy gradient > SDP)
- Control with signal temporal logical constraints <sup>4</sup>

<sup>1</sup>Williams, et al. Information theoretic MPC for model-based reinforcement learning. ICRA 2017.

<sup>2</sup>Xue, et al. Full-order sampling-based mpc for torque-level locomotion control via diffusion-style annealing. ICRA 2025.

<sup>3</sup>Pan, et al. pider: Scalable physics-informed dexterous retargeting. ArXiv 2025.

<sup>4</sup>Halder et al. Trajectory Planning with Signal Temporal Logic Costs using Deterministic Path Integral Optimization. Arxiv 2025.

# Introduction

Consider the optimization problem

$$\min_{\mathbf{u}} J(\mathbf{u}) \in \mathbb{R}_{\geq 0}. \quad (1)$$

# Introduction

Consider the optimization problem

$$\min_{\mathbf{u}} J(\mathbf{u}) \in \mathbb{R}_{\geq 0}. \quad (1)$$

The iteration formula of MPPI is

$$\mathbf{u}_{out} = \frac{\sum_{i=1}^N \mathbf{u}_i \exp(-J(\mathbf{u}_i)/\lambda)}{\sum_{i=1}^N \exp(-J(\mathbf{u}_i)/\lambda)}, \quad (2)$$

where  $\lambda$  is a hyperparameter (called temperature from simulated annealing) and  $\{\mathbf{u}_i\}_{i=1}^N$  are i.i.d. samples from the following Gaussian distribution  $\mathcal{N}(\mathbf{u}_{in}, \mathbf{\Sigma})$ , with the current controller  $\mathbf{u}_{in}$  and  $\mathbf{\Sigma} \succ 0$ .

## Derive Single MPPI Iteration Based on KL Control<sup>5</sup>

Let  $q(\mathbf{u})$  be a given probability density (for  $\mathbf{u}_{in}$ ) on  $\mathbb{R}^k$ . Let  $J : \mathbb{R}^k \rightarrow \mathbb{R}$  be measurable and  $\lambda > 0$ . We consider the optimization problem over probability densities  $p(\mathbf{u})$ :

$$\begin{aligned} \min_p \quad & \int p(\mathbf{u}) J(\mathbf{u}) d\mathbf{u} + \lambda \int p(\mathbf{u}) \log \frac{p(\mathbf{u})}{q(\mathbf{u})} d\mathbf{u} \\ \text{s.t.} \quad & \int p(\mathbf{u}) d\mathbf{u} = 1. \end{aligned} \tag{3}$$

---

<sup>5</sup>Evangelos & Todorov. Relative entropy and free energy dualities: Connections to path integral and kl control. CDC 2012.

## Derive Single MPPI Iteration Based on KL Control<sup>5</sup>

Let  $q(\mathbf{u})$  be a given probability density (for  $\mathbf{u}_{in}$ ) on  $\mathbb{R}^k$ . Let  $J : \mathbb{R}^k \rightarrow \mathbb{R}$  be measurable and  $\lambda > 0$ . We consider the optimization problem over probability densities  $p(\mathbf{u})$ :

$$\begin{aligned} \min_p \quad & \int p(\mathbf{u}) J(\mathbf{u}) d\mathbf{u} + \lambda \int p(\mathbf{u}) \log \frac{p(\mathbf{u})}{q(\mathbf{u})} d\mathbf{u} \\ \text{s.t.} \quad & \int p(\mathbf{u}) d\mathbf{u} = 1. \end{aligned} \tag{3}$$

Define

$$p^*(\mathbf{u}) := \frac{1}{\mathbb{E}_q \left[ \exp \left( -\frac{1}{\lambda} J(\mathbf{u}) \right) \right]} q(\mathbf{u}) \exp \left( -\frac{1}{\lambda} J(\mathbf{u}) \right). \tag{4}$$

---

<sup>5</sup>Evangelos & Todorov. Relative entropy and free energy dualities: Connections to path integral and kl control. CDC 2012.



## Derive Single MPPI Iteration Based on KL Control<sup>5</sup>

Let  $q(\mathbf{u})$  be a given probability density (for  $\mathbf{u}_{in}$ ) on  $\mathbb{R}^k$ . Let  $J : \mathbb{R}^k \rightarrow \mathbb{R}$  be measurable and  $\lambda > 0$ . We consider the optimization problem over probability densities  $p(\mathbf{u})$ :

$$\begin{aligned} \min_p \quad & \int p(\mathbf{u}) J(\mathbf{u}) d\mathbf{u} + \lambda \int p(\mathbf{u}) \log \frac{p(\mathbf{u})}{q(\mathbf{u})} d\mathbf{u} \\ \text{s.t.} \quad & \int p(\mathbf{u}) d\mathbf{u} = 1. \end{aligned} \tag{3}$$

Define

$$p^*(\mathbf{u}) := \frac{1}{\mathbb{E}_q \left[ \exp \left( -\frac{1}{\lambda} J(\mathbf{u}) \right) \right]} q(\mathbf{u}) \exp \left( -\frac{1}{\lambda} J(\mathbf{u}) \right). \tag{4}$$

**Goal:** prove that  $p^*$  is the unique minimizer of (3).

---

<sup>5</sup>Evangelos & Todorov. Relative entropy and free energy dualities: Connections to path integral and kl control. CDC 2012.

## Variation Calculus

**Proof.** It can be proved that (3) is a strictly convex infinite-dimensional optimization problem. Then, the feasible stationary point of its Lagrange function is a unique minimizer. Define Lagrangian

$$\mathcal{L}(p, \eta) = \int p(\mathbf{u}) J(\mathbf{u}) d\mathbf{u} + \lambda \int p(\mathbf{u}) \log \frac{p(\mathbf{u})}{q(\mathbf{u})} d\mathbf{u} + \eta \left( \int p(\mathbf{u}) d\mathbf{u} - 1 \right), \quad (5)$$

where  $\eta \in \mathbb{R}$  is a Lagrange multiplier.

## Variation Calculus

**Proof.** It can be proved that (3) is a strictly convex infinite-dimensional optimization problem. Then, the feasible stationary point of its Lagrange function is a unique minimizer. Define Lagrangian

$$\mathcal{L}(p, \eta) = \int p(\mathbf{u})J(\mathbf{u}) d\mathbf{u} + \lambda \int p(\mathbf{u}) \log \frac{p(\mathbf{u})}{q(\mathbf{u})} d\mathbf{u} + \eta \left( \int p(\mathbf{u}) d\mathbf{u} - 1 \right), \quad (5)$$

where  $\eta \in \mathbb{R}$  is a Lagrange multiplier. We compute stationarity with respect to  $p(\mathbf{u})$ . Let  $p_\epsilon = p + \epsilon h$  with  $\int h(\mathbf{u}) d\mathbf{u} = 0$ .

Using  $\frac{d}{dx}(x \log x) = 1 + \log x$ , we obtain

$$\left. \frac{d}{d\epsilon} \right|_{\epsilon=0} \mathcal{L}(p_\epsilon, \eta) = \int h(\mathbf{u}) \left[ J(\mathbf{u}) + \lambda(1 + \log p(\mathbf{u}) - \log q(\mathbf{u})) + \eta \right] d\mathbf{u}.$$

## Variation Calculus

**Proof.** It can be proved that (3) is a strictly convex infinite-dimensional optimization problem. Then, the feasible stationary point of its Lagrange function is a unique minimizer. Define Lagrangian

$$\mathcal{L}(p, \eta) = \int p(\mathbf{u}) J(\mathbf{u}) d\mathbf{u} + \lambda \int p(\mathbf{u}) \log \frac{p(\mathbf{u})}{q(\mathbf{u})} d\mathbf{u} + \eta \left( \int p(\mathbf{u}) d\mathbf{u} - 1 \right), \quad (5)$$

where  $\eta \in \mathbb{R}$  is a Lagrange multiplier. We compute stationarity with respect to  $p(\mathbf{u})$ . Let  $p_\epsilon = p + \epsilon h$  with  $\int h(\mathbf{u}) d\mathbf{u} = 0$ .

Using  $\frac{d}{dx}(x \log x) = 1 + \log x$ , we obtain

$$\left. \frac{d}{d\epsilon} \right|_{\epsilon=0} \mathcal{L}(p_\epsilon, \eta) = \int h(\mathbf{u}) \left[ J(\mathbf{u}) + \lambda(1 + \log p(\mathbf{u}) - \log q(\mathbf{u})) + \eta \right] d\mathbf{u}.$$

For this to vanish for all admissible  $h$ , the bracket must be constant:

$$J(\mathbf{u}) + \lambda(1 + \log p(\mathbf{u}) - \log q(\mathbf{u})) = c. \quad (6)$$

## Solve the Stationarity Condition

Rearranging,

$$\log p(\mathbf{u}) = \log q(\mathbf{u}) - \frac{1}{\lambda} J(\mathbf{u}) + \frac{c - \lambda}{\lambda}.$$

## Solve the Stationarity Condition

Rearranging,

$$\log p(\mathbf{u}) = \log q(\mathbf{u}) - \frac{1}{\lambda} J(\mathbf{u}) + \frac{c - \lambda}{\lambda}.$$

Exponentiating,

$$p(\mathbf{u}) = e^{\frac{c-\lambda}{\lambda}} q(\mathbf{u}) \exp\left(-\frac{1}{\lambda} J(\mathbf{u})\right).$$

## Solve the Stationarity Condition

Rearranging,

$$\log p(\mathbf{u}) = \log q(\mathbf{u}) - \frac{1}{\lambda} J(\mathbf{u}) + \frac{c - \lambda}{\lambda}.$$

Exponentiating,

$$p(\mathbf{u}) = e^{\frac{c-\lambda}{\lambda}} q(\mathbf{u}) \exp\left(-\frac{1}{\lambda} J(\mathbf{u})\right).$$

Imposing normalization  $\int p = 1$  gives

$$e^{\frac{c-\lambda}{\lambda}} = \frac{1}{\mathbb{E}_q\left[\exp\left(-\frac{1}{\lambda} J(\mathbf{u})\right)\right]},$$

## Solve the Stationarity Condition

Rearranging,

$$\log p(\mathbf{u}) = \log q(\mathbf{u}) - \frac{1}{\lambda} J(\mathbf{u}) + \frac{c - \lambda}{\lambda}.$$

Exponentiating,

$$p(\mathbf{u}) = e^{\frac{c-\lambda}{\lambda}} q(\mathbf{u}) \exp\left(-\frac{1}{\lambda} J(\mathbf{u})\right).$$

Imposing normalization  $\int p = 1$  gives

$$e^{\frac{c-\lambda}{\lambda}} = \frac{1}{\mathbb{E}_q\left[\exp\left(-\frac{1}{\lambda} J(\mathbf{u})\right)\right]},$$

so

$$p(\mathbf{u}) = \frac{1}{\mathbb{E}_q\left[\exp\left(-\frac{1}{\lambda} J(\mathbf{u})\right)\right]} q(\mathbf{u}) \exp\left(-\frac{1}{\lambda} J(\mathbf{u})\right) = p^*(\mathbf{u}).$$



## From Optimal Distribution to Optimal Controller

KL-control yields an *optimal distribution*  $p^*(\mathbf{u})$ , but controller implementation must output a deterministic value  $\bar{\mathbf{u}}$ . Adopt the posterior squared-loss criterion

$$\bar{\mathbf{u}}^* \in \arg \min_{\bar{\mathbf{u}} \in \mathbb{R}^{mH}} \mathbb{E}_{p^*}[\|\mathbf{u} - \bar{\mathbf{u}}\|_2^2]. \quad (7)$$

## From Optimal Distribution to Optimal Controller

KL-control yields an *optimal distribution*  $p^*(\mathbf{u})$ , but controller implementation must output a deterministic value  $\bar{\mathbf{u}}$ . Adopt the posterior squared-loss criterion

$$\bar{\mathbf{u}}^* \in \arg \min_{\bar{\mathbf{u}} \in \mathbb{R}^{mH}} \mathbb{E}_{p^*}[\|\mathbf{u} - \bar{\mathbf{u}}\|_2^2]. \quad (7)$$

Expand the risk:

$$\mathbb{E}_{p^*}[\|\mathbf{u} - \bar{\mathbf{u}}\|_2^2] = \mathbb{E}_{p^*}[\|\mathbf{u}\|_2^2] - 2\bar{\mathbf{u}}^\top \mathbb{E}_{p^*}[\mathbf{u}] + \|\bar{\mathbf{u}}\|_2^2. \quad (8)$$

## From Optimal Distribution to Optimal Controller

KL-control yields an *optimal distribution*  $p^*(\mathbf{u})$ , but controller implementation must output a deterministic value  $\bar{\mathbf{u}}$ . Adopt the posterior squared-loss criterion

$$\bar{\mathbf{u}}^* \in \arg \min_{\bar{\mathbf{u}} \in \mathbb{R}^{mH}} \mathbb{E}_{p^*}[\|\mathbf{u} - \bar{\mathbf{u}}\|_2^2]. \quad (7)$$

Expand the risk:

$$\mathbb{E}_{p^*}[\|\mathbf{u} - \bar{\mathbf{u}}\|_2^2] = \mathbb{E}_{p^*}[\|\mathbf{u}\|_2^2] - 2\bar{\mathbf{u}}^\top \mathbb{E}_{p^*}[\mathbf{u}] + \|\bar{\mathbf{u}}\|_2^2. \quad (8)$$

Differentiate w.r.t.  $\bar{\mathbf{u}}$ :

$$\nabla_{\bar{\mathbf{u}}} = -2\mathbb{E}_{p^*}[\mathbf{u}] + 2\bar{\mathbf{u}}. \quad (9)$$

Setting  $\nabla_{\bar{\mathbf{u}}} = 0$  gives

$$\bar{\mathbf{u}}^* = \mathbb{E}_{p^*}[\mathbf{u}].$$

Since the Hessian is  $2I \succ 0$ , this minimizer is unique.

# Convergence of MPPI for Quadratic Programming

Consider a QP

$$\min_{\mathbf{u}} J(\mathbf{u}) = \mathbf{u}^\top \mathbf{D} \mathbf{u} + \mathbf{u}^\top \mathbf{d}, \quad (10)$$

with  $\mathbf{D} \succ 0$ . Draw  $N$  i.i.d. samples  $\mathbf{u}_i \sim q = \mathcal{N}(\mathbf{u}_{in}, \mathbf{\Sigma})$  with  $\mathbf{\Sigma} \succ 0$ .

---

<sup>6</sup>Yi et al. CoVO-MPC: Theoretical Analysis of Sampling-based MPC and Optimal Covariance Design. L4DC 2024.

# Convergence of MPPI for Quadratic Programming

Consider a QP

$$\min_{\mathbf{u}} J(\mathbf{u}) = \mathbf{u}^\top \mathbf{D} \mathbf{u} + \mathbf{u}^\top \mathbf{d}, \quad (10)$$

with  $\mathbf{D} \succ 0$ . Draw  $N$  i.i.d. samples  $\mathbf{u}_i \sim q = \mathcal{N}(\mathbf{u}_{in}, \mathbf{\Sigma})$  with  $\mathbf{\Sigma} \succ 0$ . Consider the MPPI update

$$\hat{\mathbf{u}}_{\text{out}} = \frac{\sum_{i=1}^N \mathbf{u}_i \exp(-J(\mathbf{u}_i)/\lambda)}{\sum_{i=1}^N \exp(-J(\mathbf{u}_i)/\lambda)} \text{ and } \mathbf{u}_{\text{out}} = \frac{\mathbb{E}_q[\mathbf{u} \exp(-\frac{1}{\lambda}J(\mathbf{u}))]}{\mathbb{E}_q[\exp(-\frac{1}{\lambda}J(\mathbf{u}))]}. \quad (11)$$

---

<sup>6</sup>Yi et al. CoVO-MPC: Theoretical Analysis of Sampling-based MPC and Optimal Covariance Design. L4DC 2024.

# Convergence of MPPI for Quadratic Programming

Consider a QP

$$\min_{\mathbf{u}} J(\mathbf{u}) = \mathbf{u}^\top \mathbf{D} \mathbf{u} + \mathbf{u}^\top \mathbf{d}, \quad (10)$$

with  $\mathbf{D} \succ 0$ . Draw  $N$  i.i.d. samples  $\mathbf{u}_i \sim q = \mathcal{N}(\mathbf{u}_{in}, \mathbf{\Sigma})$  with  $\mathbf{\Sigma} \succ 0$ . Consider the MPPI update

$$\hat{\mathbf{u}}_{out} = \frac{\sum_{i=1}^N \mathbf{u}_i \exp(-J(\mathbf{u}_i)/\lambda)}{\sum_{i=1}^N \exp(-J(\mathbf{u}_i)/\lambda)} \text{ and } \mathbf{u}_{out} = \frac{\mathbb{E}_q[\mathbf{u} \exp(-\frac{1}{\lambda}J(\mathbf{u}))]}{\mathbb{E}_q[\exp(-\frac{1}{\lambda}J(\mathbf{u}))]}. \quad (11)$$

**Theorem 1.**<sup>6</sup> Consider the minimizer  $\mathbf{u}^* = \frac{-1}{2} \mathbf{d} \mathbf{D}^{-1}$  of (10). We have

$$\hat{\mathbf{u}}_{out} \xrightarrow{P} \mathbf{u}_{out}, \quad (12)$$

and

$$\mathbf{u}_{out} - \mathbf{u}^* \xrightarrow{P} (\mathbf{I} + 2\lambda \mathbf{\Sigma} \mathbf{D})^{-1} (\mathbf{u}_{in} - \mathbf{u}^*). \quad (13)$$

---

<sup>6</sup>Yi et al. CoVO-MPC: Theoretical Analysis of Sampling-based MPC and Optimal Covariance Design. L4DC 2024.

## Step 1: Write $p^\star$ exactly

**Proof.** Define

$$Z := \mathbb{E}_q \left[ \exp \left( - \frac{1}{\lambda} J(\mathbf{u}) \right) \right] = \int_{\mathbb{R}^k} q(\mathbf{u}) \exp \left( - \frac{1}{\lambda} J(\mathbf{u}) \right) d\mathbf{u}. \quad (14)$$

Then the optimal distribution satisfies

$$p^\star(\mathbf{u}) = \frac{1}{Z} q(\mathbf{u}) \exp \left( - \frac{1}{\lambda} J(\mathbf{u}) \right), \quad \mathbf{u}_{out} = \mathbb{E}_{p^\star}[\mathbf{u}]. \quad (15)$$

## Step 1: Write $p^\star$ exactly

**Proof.** Define

$$Z := \mathbb{E}_q \left[ \exp \left( - \frac{1}{\lambda} J(\mathbf{u}) \right) \right] = \int_{\mathbb{R}^k} q(\mathbf{u}) \exp \left( - \frac{1}{\lambda} J(\mathbf{u}) \right) d\mathbf{u}. \quad (14)$$

Then the optimal distribution satisfies

$$p^\star(\mathbf{u}) = \frac{1}{Z} q(\mathbf{u}) \exp \left( - \frac{1}{\lambda} J(\mathbf{u}) \right), \quad \mathbf{u}_{out} = \mathbb{E}_{p^\star}[\mathbf{u}]. \quad (15)$$

Because  $q(\mathbf{u}) = \mathcal{N}(\mathbf{u}_{in}, \mathbf{\Sigma})$ , then

$$q(\mathbf{u}) = \frac{1}{(2\pi)^{k/2} |\mathbf{\Sigma}|^{1/2}} \exp \left( - \frac{1}{2} (\mathbf{u} - \mathbf{u}_{in})^\top \mathbf{\Sigma}^{-1} (\mathbf{u} - \mathbf{u}_{in}) \right). \quad (16)$$



## Step 1: Write $p^*$ exactly

**Proof.** Define

$$Z := \mathbb{E}_q \left[ \exp \left( -\frac{1}{\lambda} J(\mathbf{u}) \right) \right] = \int_{\mathbb{R}^k} q(\mathbf{u}) \exp \left( -\frac{1}{\lambda} J(\mathbf{u}) \right) d\mathbf{u}. \quad (14)$$

Then the optimal distribution satisfies

$$p^*(\mathbf{u}) = \frac{1}{Z} q(\mathbf{u}) \exp \left( -\frac{1}{\lambda} J(\mathbf{u}) \right), \quad \mathbf{u}_{out} = \mathbb{E}_{p^*}[\mathbf{u}]. \quad (15)$$

Because  $q(\mathbf{u}) = \mathcal{N}(\mathbf{u}_{in}, \mathbf{\Sigma})$ , then

$$q(\mathbf{u}) = \frac{1}{(2\pi)^{k/2} |\mathbf{\Sigma}|^{1/2}} \exp \left( -\frac{1}{2} (\mathbf{u} - \mathbf{u}_{in})^\top \mathbf{\Sigma}^{-1} (\mathbf{u} - \mathbf{u}_{in}) \right). \quad (16)$$

Using  $J(\mathbf{u}) = \mathbf{u}^\top \mathbf{D} \mathbf{u} + \mathbf{u}^\top \mathbf{d}$ , we obtain the exact product

$$q(\mathbf{u}) \exp \left( -\frac{1}{\lambda} J(\mathbf{u}) \right) = \frac{1}{(2\pi)^{k/2} |\mathbf{\Sigma}|^{1/2}} \exp \left( -\frac{1}{2} \mathbf{u}^\top \mathbf{A} \mathbf{u} + \mathbf{u}^\top \mathbf{b} - c_0 \right), \quad (17)$$

where

$$\mathbf{A} := \mathbf{\Sigma}^{-1} + \frac{2}{\lambda} \mathbf{D}, \quad \mathbf{b} := \mathbf{\Sigma}^{-1} \mathbf{u}_{in} - \frac{1}{\lambda} \mathbf{d}, \quad c_0 := \frac{1}{2} \mathbf{u}_{in}^\top \mathbf{\Sigma}^{-1} \mathbf{u}_{in}. \quad (18)$$

## Step 2: Complete the square and normalize

Complete the square with  $\boldsymbol{\mu} := \mathbf{A}^{-1}\mathbf{b}$ :

$$-\frac{1}{2}\mathbf{u}^\top \mathbf{A}\mathbf{u} + \mathbf{u}^\top \mathbf{b} = -\frac{1}{2}(\mathbf{u} - \boldsymbol{\mu})^\top \mathbf{A}(\mathbf{u} - \boldsymbol{\mu}) + \frac{1}{2}\mathbf{b}^\top \mathbf{A}^{-1}\mathbf{b}. \quad (19)$$

## Step 2: Complete the square and normalize

Complete the square with  $\boldsymbol{\mu} := \mathbf{A}^{-1}\mathbf{b}$ :

$$-\frac{1}{2}\mathbf{u}^\top \mathbf{A} \mathbf{u} + \mathbf{u}^\top \mathbf{b} = -\frac{1}{2}(\mathbf{u} - \boldsymbol{\mu})^\top \mathbf{A}(\mathbf{u} - \boldsymbol{\mu}) + \frac{1}{2}\mathbf{b}^\top \mathbf{A}^{-1}\mathbf{b}. \quad (19)$$

Hence

$$p^*(\mathbf{u}) = \frac{1}{Z} \cdot \frac{1}{(2\pi)^{k/2} |\boldsymbol{\Sigma}|^{1/2}} \exp\left(\frac{1}{2}\mathbf{b}^\top \mathbf{A}^{-1}\mathbf{b} - c_0\right) \exp\left(-\frac{1}{2}(\mathbf{u} - \boldsymbol{\mu})^\top \mathbf{A}(\mathbf{u} - \boldsymbol{\mu})\right). \quad (20)$$

## Step 2: Complete the square and normalize

Complete the square with  $\boldsymbol{\mu} := \mathbf{A}^{-1}\mathbf{b}$ :

$$-\frac{1}{2}\mathbf{u}^\top \mathbf{A} \mathbf{u} + \mathbf{u}^\top \mathbf{b} = -\frac{1}{2}(\mathbf{u} - \boldsymbol{\mu})^\top \mathbf{A}(\mathbf{u} - \boldsymbol{\mu}) + \frac{1}{2}\mathbf{b}^\top \mathbf{A}^{-1}\mathbf{b}. \quad (19)$$

Hence

$$p^*(\mathbf{u}) = \frac{1}{Z} \cdot \frac{1}{(2\pi)^{k/2} |\boldsymbol{\Sigma}|^{1/2}} \exp\left(\frac{1}{2}\mathbf{b}^\top \mathbf{A}^{-1}\mathbf{b} - c_0\right) \exp\left(-\frac{1}{2}(\mathbf{u} - \boldsymbol{\mu})^\top \mathbf{A}(\mathbf{u} - \boldsymbol{\mu})\right). \quad (20)$$

After a long derivation,

$$Z = \int_{\mathbb{R}^k} q(\mathbf{u}) \exp\left(-\frac{1}{\lambda} J(\mathbf{u})\right) d\mathbf{u} = \frac{|\mathbf{A}^{-1}|^{1/2}}{|\boldsymbol{\Sigma}|^{1/2}} \exp\left(\frac{1}{2}\mathbf{b}^\top \mathbf{A}^{-1}\mathbf{b} - \frac{1}{2}\mathbf{u}_{in}^\top \boldsymbol{\Sigma}^{-1}\mathbf{u}_{in}\right). \quad (21)$$

## Step 2: Complete the square and normalize

Complete the square with  $\boldsymbol{\mu} := \mathbf{A}^{-1}\mathbf{b}$ :

$$-\frac{1}{2}\mathbf{u}^\top \mathbf{A}\mathbf{u} + \mathbf{u}^\top \mathbf{b} = -\frac{1}{2}(\mathbf{u} - \boldsymbol{\mu})^\top \mathbf{A}(\mathbf{u} - \boldsymbol{\mu}) + \frac{1}{2}\mathbf{b}^\top \mathbf{A}^{-1}\mathbf{b}. \quad (19)$$

Hence

$$p^*(\mathbf{u}) = \frac{1}{Z} \cdot \frac{1}{(2\pi)^{k/2} |\boldsymbol{\Sigma}|^{1/2}} \exp\left(\frac{1}{2}\mathbf{b}^\top \mathbf{A}^{-1}\mathbf{b} - c_0\right) \exp\left(-\frac{1}{2}(\mathbf{u} - \boldsymbol{\mu})^\top \mathbf{A}(\mathbf{u} - \boldsymbol{\mu})\right). \quad (20)$$

After a long derivation,

$$Z = \int_{\mathbb{R}^k} q(\mathbf{u}) \exp\left(-\frac{1}{\lambda} J(\mathbf{u})\right) d\mathbf{u} = \frac{|\mathbf{A}^{-1}|^{1/2}}{|\boldsymbol{\Sigma}|^{1/2}} \exp\left(\frac{1}{2}\mathbf{b}^\top \mathbf{A}^{-1}\mathbf{b} - \frac{1}{2}\mathbf{u}_{in}^\top \boldsymbol{\Sigma}^{-1}\mathbf{u}_{in}\right). \quad (21)$$

Substituting this  $Z$  back to (20) yields the fully normalized Gaussian form

$$p^*(\mathbf{u}) = \frac{|\mathbf{A}|^{1/2}}{(2\pi)^{k/2}} \exp\left(-\frac{1}{2}(\mathbf{u} - \boldsymbol{\mu})^\top \mathbf{A}(\mathbf{u} - \boldsymbol{\mu})\right) = \mathcal{N}(\boldsymbol{\mu}, \mathbf{A}^{-1}). \quad (22)$$

In particular,

$$\mathbf{u}_{out} = \mathbb{E}_{p^*}[\mathbf{u}] = \boldsymbol{\mu} = \left(\boldsymbol{\Sigma}^{-1} + \frac{2}{\lambda}\mathbf{D}\right)^{-1} \left(\boldsymbol{\Sigma}^{-1}\mathbf{u}_{in} - \frac{1}{\lambda}\mathbf{d}\right). \quad (23)$$

### Step 3: Express the mean as a contraction toward $\mathbf{u}^\star$

Recall

$$\mathbf{u}_{out} = \left( \boldsymbol{\Sigma}^{-1} + \frac{2}{\lambda} \mathbf{D} \right)^{-1} \left( \boldsymbol{\Sigma}^{-1} \mathbf{u}_{in} - \frac{1}{\lambda} \mathbf{d} \right). \quad (24)$$

### Step 3: Express the mean as a contraction toward $\mathbf{u}^*$

Recall

$$\mathbf{u}_{out} = \left( \mathbf{\Sigma}^{-1} + \frac{2}{\lambda} \mathbf{D} \right)^{-1} \left( \mathbf{\Sigma}^{-1} \mathbf{u}_{in} - \frac{1}{\lambda} \mathbf{d} \right). \quad (24)$$

Since  $\nabla J(\mathbf{u}^*) = 0$  yeilds  $\mathbf{d} = -2\mathbf{D}\mathbf{u}^*$ . Then  $-\frac{1}{\lambda}\mathbf{d} = \frac{2}{\lambda}\mathbf{D}\mathbf{u}^*$ .

### Step 3: Express the mean as a contraction toward $\mathbf{u}^*$

Recall

$$\mathbf{u}_{out} = \left( \mathbf{\Sigma}^{-1} + \frac{2}{\lambda} \mathbf{D} \right)^{-1} \left( \mathbf{\Sigma}^{-1} \mathbf{u}_{in} - \frac{1}{\lambda} \mathbf{d} \right). \quad (24)$$

Since  $\nabla J(\mathbf{u}^*) = 0$  yields  $\mathbf{d} = -2\mathbf{D}\mathbf{u}^*$ . Then  $-\frac{1}{\lambda}\mathbf{d} = \frac{2}{\lambda}\mathbf{D}\mathbf{u}^*$ . Substitute and regroup:

$$\mathbf{u}_{out} = \left( \mathbf{\Sigma}^{-1} + \frac{2}{\lambda} \mathbf{D} \right)^{-1} \left( \mathbf{\Sigma}^{-1} \mathbf{u}_{in} + \frac{2}{\lambda} \mathbf{D} \mathbf{u}^* \right) \quad (25)$$

$$= (\lambda \mathbf{I} + 2\mathbf{\Sigma D})^{-1} \left( \lambda \mathbf{u}_{in} + 2\mathbf{\Sigma D} \mathbf{u}^* \right) \quad (26)$$

$$= (\lambda \mathbf{I} + 2\mathbf{\Sigma D})^{-1} \left( \lambda \mathbf{u}_{in} + 2\mathbf{\Sigma D} \mathbf{u}_{in} - 2\mathbf{\Sigma D} \mathbf{u}_{in} + 2\mathbf{\Sigma D} \mathbf{u}^* \right) \quad (27)$$

$$= \mathbf{u}_{in} + (\lambda \mathbf{I} + 2\mathbf{\Sigma D})^{-1} 2\mathbf{\Sigma D} (\mathbf{u}^* - \mathbf{u}_{in}). \quad (28)$$



### Step 3: Express the mean as a contraction toward $\mathbf{u}^*$

Recall

$$\mathbf{u}_{out} = \left( \mathbf{\Sigma}^{-1} + \frac{2}{\lambda} \mathbf{D} \right)^{-1} \left( \mathbf{\Sigma}^{-1} \mathbf{u}_{in} - \frac{1}{\lambda} \mathbf{d} \right). \quad (24)$$

Since  $\nabla J(\mathbf{u}^*) = 0$  yields  $\mathbf{d} = -2\mathbf{D}\mathbf{u}^*$ . Then  $-\frac{1}{\lambda}\mathbf{d} = \frac{2}{\lambda}\mathbf{D}\mathbf{u}^*$ . Substitute and regroup:

$$\mathbf{u}_{out} = \left( \mathbf{\Sigma}^{-1} + \frac{2}{\lambda} \mathbf{D} \right)^{-1} \left( \mathbf{\Sigma}^{-1} \mathbf{u}_{in} + \frac{2}{\lambda} \mathbf{D} \mathbf{u}^* \right) \quad (25)$$

$$= (\lambda \mathbf{I} + 2\mathbf{\Sigma D})^{-1} \left( \lambda \mathbf{u}_{in} + 2\mathbf{\Sigma D} \mathbf{u}^* \right) \quad (26)$$

$$= (\lambda \mathbf{I} + 2\mathbf{\Sigma D})^{-1} \left( \lambda \mathbf{u}_{in} + 2\mathbf{\Sigma D} \mathbf{u}_{in} - 2\mathbf{\Sigma D} \mathbf{u}_{in} + 2\mathbf{\Sigma D} \mathbf{u}^* \right) \quad (27)$$

$$= \mathbf{u}_{in} + (\lambda \mathbf{I} + 2\mathbf{\Sigma D})^{-1} 2\mathbf{\Sigma D} (\mathbf{u}^* - \mathbf{u}_{in}). \quad (28)$$

Therefore,

$$\mathbf{u}_{out} - \mathbf{u}^* = (\mathbf{I} + 2\lambda \mathbf{\Sigma D})^{-1} (\mathbf{u}_{in} - \mathbf{u}^*).$$

## Step 4: Convergence in probability and Slutsky

Let the MPPI estimator be

$$\mathbf{u}_{out}^{(N)} = \frac{\frac{1}{N} \sum_{i=1}^N \mathbf{u}_i w_i}{\frac{1}{N} \sum_{i=1}^N w_i}, \quad w_i := \exp\left(-\frac{1}{\lambda} J(\mathbf{u}_i)\right), \quad \mathbf{u}_i \stackrel{\text{i.i.d.}}{\sim} q. \quad (29)$$

## Step 4: Convergence in probability and Slutsky

Let the MPPI estimator be

$$\mathbf{u}_{out}^{(N)} = \frac{\frac{1}{N} \sum_{i=1}^N \mathbf{u}_i w_i}{\frac{1}{N} \sum_{i=1}^N w_i}, \quad w_i := \exp\left(-\frac{1}{\lambda} J(\mathbf{u}_i)\right), \quad \mathbf{u}_i \stackrel{\text{i.i.d.}}{\sim} q. \quad (29)$$

Then by the weak LLN,

$$\frac{1}{N} \sum_{i=1}^N w_i \xrightarrow{P} \mathbb{E}_q[w], \quad \frac{1}{N} \sum_{i=1}^N \mathbf{u}_i w_i \xrightarrow{P} \mathbb{E}_q[\mathbf{u}w]. \quad (30)$$

## Step 4: Convergence in probability and Slutsky

Let the MPPI estimator be

$$\mathbf{u}_{out}^{(N)} = \frac{\frac{1}{N} \sum_{i=1}^N \mathbf{u}_i w_i}{\frac{1}{N} \sum_{i=1}^N w_i}, \quad w_i := \exp\left(-\frac{1}{\lambda} J(\mathbf{u}_i)\right), \quad \mathbf{u}_i \stackrel{\text{i.i.d.}}{\sim} q. \quad (29)$$

Then by the weak LLN,

$$\frac{1}{N} \sum_{i=1}^N w_i \xrightarrow{P} \mathbb{E}_q[w], \quad \frac{1}{N} \sum_{i=1}^N \mathbf{u}_i w_i \xrightarrow{P} \mathbb{E}_q[\mathbf{u}w]. \quad (30)$$

Then, Slutsky's theorem yields

$$\hat{\mathbf{u}}_{out} \xrightarrow{P} \frac{\mathbb{E}_q[\mathbf{u}w]}{\mathbb{E}_q[w]} = \mathbb{E}_{p^*}[\mathbf{u}] = \mathbf{u}_{out}. \quad (31)$$